## 곱셉에서의 지수 법칙

### 같은 밑을 가진 거듭제곱

### 3x * 3x * 3x

`3x * 3x * 3x === (3 * 3 * 3)* x * x * x`

`(3 * 3 * 3)* x * x * x === 3 ** 3 * x ** 3`

왜 이 법칙이 성립하는가?

`3x * 3x * 3x` 는 `(3x) ** 3` 이기 때문

### 6 ** 3 * 6 ** 6

`6 ** 3 * 6 ** 6 === (6 * 6 * 6) * (6 * 6 * 6 * 6 * 6 * 6)`

`6 ** 3 * 6 ** 6 === 6 ** (3 + 6)`

`6 ** (3 + 6) === 6 ** 9`

### x ** 2 * x ** 4

`x ** 6`

### x ** a * x ** b

`x ** (a + b)`

### (x * y) ** a

`x ** a * y ** a`

### 거듭제곱의 거듭 제곱

`(a ** 3) ** 4`

`(a ** 3) ** 4 === a ** 3 * a ** 3 * a ** 3 * a ** 3`

`a ** 3 * a ** 3 * a ** 3 * a ** 3 === a ** (3 + 3 + 3 + 3)`

`a ** (3 + 3 + 3 + 3) === a ** (3 * 4)`

`a ** (3 * 4) === a ** 12`

### (x ** a) ** b

`x ** (a * b)`
